LeanYjs/ItemOrder.lean
@@ -3,41 +3,130 @@ import LeanYjs.ActorId
 import LeanYjs.ItemOriginOrder
 
 import Mathlib.Tactic.ApplyAt
+import Mathlib.Tactic.Tauto
 import Mathlib.Data.Nat.Basic
 
 def max4 (x y z w : Nat) : Nat :=
   max (max x y) (max z w)
 
 mutual
-inductive YjsLt {A : Type} : Nat -> YjsPtr A -> YjsPtr A -> Prop where
-  | ltConflict h i1 i2 : ConflictLt h i1 i2 -> YjsLt (h + 1) i1 i2
-  | ltOriginOrder i1 i2 : OriginLt _ i1 i2 -> YjsLt 0 i1 i2
-  | ltTrans h1 h2 x y z: YjsLt h1 x y -> YjsLt h2 y z -> YjsLt (max h1 h2 + 1) x z
+  inductive YjsLt {A : Type} (P : @ClosedPredicate A) : Nat -> YjsPtr A -> YjsPtr A -> Prop where
+    | ltConflict h i1 i2 : ConflictLt P h i1 i2 -> YjsLt P (h + 1) i1 i2
+    | ltOriginOrder i1 i2 : OriginLt _ P i1 i2 -> YjsLt P 0 i1 i2
+    | ltTrans h1 h2 x (y : YjsItem A) z: YjsLt P h1 x y -> YjsLt P h2 y z -> YjsLt P (max h1 h2 + 1) x z
 
-inductive ConflictLt {A : Type} : Nat -> YjsPtr A -> YjsPtr A -> Prop where
-  | ltOriginDiff h1 h2 h3 h4 l1 l2 r1 r2 id1 id2 c1 c2 :
-    YjsLt h1 l2 l1
-    -> YjsLt h2 (YjsItem.item l1 r1 id1 c1) r2
-    -> YjsLt h3 l1 (YjsItem.item l2 r2 id2 c2)
-    -> YjsLt h4 (YjsItem.item l2 r2 id2 c2) r1
-    -> ConflictLt (max4 h1 h2 h3 h4 + 1) (YjsItem.item l1 r1 id1 c1) (YjsItem.item l2 r2 id2 c2)
-  | ltOriginSame h1 h2 l r1 r2 id1 id2 (c1 c2 : A) :
-    YjsLt h1 (YjsItem.item l r1 id1 c1) r2
-    -> YjsLt h2 (YjsItem.item l r2 id2 c2) r1
-    -> id1 < id2
-    -> ConflictLt (max h1 h2 + 1) (YjsItem.item l r1 id1 c1) (YjsItem.item l r2 id2 c2)
+  inductive ConflictLt {A : Type} (P : @ClosedPredicate A) : Nat -> YjsPtr A -> YjsPtr A -> Prop where
+    | ltOriginDiff h1 h2 h3 h4 l1 l2 r1 r2 id1 id2 c1 c2 :
+      YjsLt P h1 l2 l1
+      -> YjsLt P h2 (YjsItem.item l1 r1 id1 c1) r2
+      -> YjsLt P h3 l1 (YjsItem.item l2 r2 id2 c2)
+      -> YjsLt P h4 (YjsItem.item l2 r2 id2 c2) r1
+      -> ConflictLt P (max4 h1 h2 h3 h4 + 1) (YjsItem.item l1 r1 id1 c1) (YjsItem.item l2 r2 id2 c2)
+    | ltOriginSame h1 h2 l r1 r2 id1 id2 (c1 c2 : A) :
+      YjsLt P h1 (YjsItem.item l r1 id1 c1) r2
+      -> YjsLt P h2 (YjsItem.item l r2 id2 c2) r1
+      -> id1 < id2
+      -> ConflictLt P (max h1 h2 + 1) (YjsItem.item l r1 id1 c1) (YjsItem.item l r2 id2 c2)
 end
 
-def YjsLeq {A : Type} (h : Nat) (x y : YjsPtr A) : Prop :=
-  x = y ∨ YjsLt h x y
+lemma yjs_lt_p1_aux {A : Type} {P : @ClosedPredicate A} {h : Nat} : forall {x y : YjsPtr A},
+  (YjsLt P h x y -> P.val x) ∧ (ConflictLt P h x y -> P.val x) := by
+    apply Nat.strongRecOn' (P := fun h => ∀ x y, (YjsLt P h x y -> P.val x) ∧ (ConflictLt P h x y -> P.val x))
+    intros n ih x y
+    constructor
+    . intro hlt
+      cases hlt with
+      | ltConflict h x y hlt =>
+        have hlt_h : h < h + 1 := by
+          omega
+        let ⟨ _, h ⟩ := ih h hlt_h x y
+        apply h ; assumption
+      | ltOriginOrder x y _ =>
+        apply origin_lt_p1; assumption
+      | ltTrans h1 h2 x y z _ _ =>
+        have hlt_h : h1 < max h1 h2 + 1 := by
+          omega
+        let ⟨ h, _ ⟩ := ih h1 hlt_h x y
+        tauto
+    . intro hlt
+      cases hlt with
+      | ltOriginDiff h1 h2 h3 h4 l1 l2 r1 r2 id1 id2 c1 c2 hlt1 hlt2 hlt3 =>
+        have hlt_h : h2 < max4 h1 h2 h3 h4 + 1 := by
+          unfold max4
+          omega
+        let ⟨ _, ih ⟩ := ih h2 hlt_h (YjsPtr.itemPtr (YjsItem.item l1 r1 id1 c1)) r2
+        tauto
+      | ltOriginSame h1 h2 l r1 r2 id1 id2 c1 c2 hlt1 hlt2 _ =>
+        have hlt_h : h1 < max h1 h2 + 1 := by
+          omega
+        let ⟨ _, ih ⟩ := ih h1 hlt_h (YjsPtr.itemPtr (YjsItem.item l r1 id1 c1)) r2
+        tauto
 
-inductive LtSequence {A : Type} : YjsPtr A -> YjsPtr A -> List (YjsPtr A) -> Prop where
-  | base : forall x, LtSequence x x []
-  | step1 : forall x y z is h, ConflictLt h x y -> LtSequence y z is -> LtSequence x z (y :: is)
-  | step2 : forall x y z is, OriginLt _ x y -> LtSequence y z is -> LtSequence x z (y :: is)
+lemma yjs_lt_p1 {A : Type} {P : @ClosedPredicate A} {h : Nat} : forall {x y : YjsPtr A},
+  YjsLt P h x y -> P.val x := by
+    intros x y hlt
+    let ⟨ h, _ ⟩ := @yjs_lt_p1_aux A P h x y
+    tauto
 
-lemma LtSequenceConcat {A : Type} {x y z : YjsPtr A} {is1 is2 : List (YjsPtr A)} :
-  LtSequence x y is1 -> LtSequence y z is2 -> LtSequence x z (is1 ++ is2) := by
+lemma conflict_lt_p1 {A : Type} {P : @ClosedPredicate A} {h : Nat} : forall {x y : YjsPtr A},
+  ConflictLt P h x y -> P.val x := by
+    intros x y hlt
+    let ⟨ _, h ⟩ := @yjs_lt_p1_aux A P h x y
+    tauto
+
+lemma yjs_lt_p2_aux {A : Type} {P : @ClosedPredicate A} {h : Nat} : forall {x y : YjsPtr A},
+  (YjsLt P h x y -> P.val y) ∧ (ConflictLt P h x y -> P.val y) := by
+    apply Nat.strongRecOn' (P := fun h => ∀ x y, (YjsLt P h x y -> P.val y) ∧ (ConflictLt P h x y -> P.val y))
+    intros n ih x y
+    constructor
+    . intro hlt
+      cases hlt with
+      | ltConflict h x y hlt =>
+        have hlt_h : h < h + 1 := by
+          omega
+        let ⟨ _, h ⟩ := ih h hlt_h x y
+        apply h ; assumption
+      | ltOriginOrder x y _ =>
+        apply origin_lt_p2; assumption
+      | ltTrans h1 h2 _ y' _ hlt1 hlt2 =>
+        have hlt_h : h2 < max h1 h2 + 1 := by
+          omega
+        let ⟨ h, _ ⟩ := ih h2 hlt_h y' y
+        tauto
+    . intro hlt
+      cases hlt with
+      | ltOriginDiff h1 h2 h3 h4 l1 l2 r1 r2 id1 id2 c1 c2 hlt1 hlt2 hlt3 =>
+        have hlt_h : h3 < max4 h1 h2 h3 h4 + 1 := by
+          unfold max4
+          omega
+        let ⟨ _, ih ⟩ := ih h3 hlt_h l1 (YjsPtr.itemPtr (YjsItem.item l2 r2 id2 c2))
+        tauto
+      | ltOriginSame h1 h2 l r1 r2 id1 id2 c1 c2 hlt1 hlt2 _ =>
+        apply yjs_lt_p1 hlt2
+
+
+lemma yjs_lt_p2 {A : Type} {P : @ClosedPredicate A} {h : Nat} : forall {x y : YjsPtr A},
+  YjsLt P h x y -> P.val y := by
+    intros x y hlt
+    let ⟨ h, _ ⟩ := @yjs_lt_p2_aux A P h x y
+    tauto
+
+lemma conflict_lt_p2 {A : Type} {P : @ClosedPredicate A} {h : Nat} : forall {x y : YjsPtr A},
+  ConflictLt P h x y -> P.val y := by
+    intros x y hlt
+    let ⟨ _, h ⟩ := @yjs_lt_p2_aux A P h x y
+    tauto
+
+def YjsLeq {A : Type} (P : @ClosedPredicate A) (h : Nat) (x y : YjsPtr A) : Prop :=
+  x = y ∨ YjsLt P h x y
+
+inductive LtSequence {A : Type} (P : @ClosedPredicate A) : YjsPtr A -> YjsPtr A -> List (YjsPtr A) -> Prop where
+  | base : forall x, LtSequence P x x []
+  | step1 : forall x y z is h, ConflictLt P h x y -> LtSequence P y z is -> LtSequence P x z (y :: is)
+  | step2 : forall x y z is, OriginLt _ P x y -> LtSequence P y z is -> LtSequence P x z (y :: is)
+
+lemma LtSequenceConcat {A : Type} {P : @ClosedPredicate A} {x y z : YjsPtr A} {is1 is2 : List (YjsPtr A)} :
+  LtSequence P x y is1 -> LtSequence P y z is2 -> LtSequence P x z (is1 ++ is2) := by
     intro lt1
     induction lt1 with
     | base x =>
@@ -55,10 +144,10 @@ lemma LtSequenceConcat {A : Type} {x y z : YjsPtr A} {is1 is2 : List (YjsPtr A)}
       assumption
 
 mutual
-def YjsLtSequence (A : Type) : forall (x y : YjsPtr A) h, YjsLt h x y ->
-  ∃ is : List (YjsPtr A), LtSequence x y is := by
+def YjsLtSequence (A : Type) (P : ClosedPredicate A): forall (x y : YjsPtr A) h, YjsLt P h x y ->
+  ∃ is : List (YjsPtr A), LtSequence P x y is := by
     intros x y h
-    apply Nat.strongRecOn' (P := fun h => ∀ x y, YjsLt h x y -> ∃ is : List (YjsPtr A), LtSequence x y is)
+    apply Nat.strongRecOn' (P := fun h => ∀ x y, YjsLt P h x y -> ∃ is : List (YjsPtr A), LtSequence P x y is)
     intros h' ih x y lt
     match lt with
     | YjsLt.ltConflict h x y _ =>
@@ -87,7 +176,3 @@ def YjsLtSequence (A : Type) : forall (x y : YjsPtr A) h, YjsLt h x y ->
           apply Exists.intro (is1 ++ is2)
           apply LtSequenceConcat <;> try assumption
 end
-
-lemma YjsInvariant A h (x y : YjsItem A) :
-  @YjsLt A h x y -> ∃ h1, @YjsLeq A h1 x (y.origin) ∨ @YjsLeq A h1 (y.origin) (x.origin) := by
-  sorry
