LeanYjs/ItemOriginOrder.lean
@@ -6,45 +6,65 @@ open Relation
 
 variable (A : Type) [BEq A]
 
+def IsItemClosed (P : YjsPtr A -> Prop) : Prop :=
+  P YjsPtr.first ∧
+  P YjsPtr.last ∧
+  (∀ (o : YjsPtr A) r id c, P (YjsItem.item o r id c) -> P o) ∧
+  (∀ o (r : YjsPtr A) id c, P (YjsItem.item o r id c) -> P r)
+
+def ClosedPredicate := { P : YjsPtr A -> Prop // IsItemClosed A P }
+
 inductive OriginLtStep : YjsPtr A -> YjsPtr A -> Prop where
   | lt_left : forall o r id c, OriginLtStep o (YjsItem.item o r id c)
   | lt_right : forall o r id c, OriginLtStep (YjsItem.item o r id c) r
   | lt_first : forall item, OriginLtStep YjsPtr.first (YjsPtr.itemPtr item)
   | lt_last : forall item, OriginLtStep (YjsPtr.itemPtr item) YjsPtr.last
+  | lt_first_last : OriginLtStep YjsPtr.first YjsPtr.last
 
 inductive OriginReachableStep : YjsPtr A -> YjsPtr A -> Prop where
   | reachable : forall o r id c, OriginReachableStep (YjsItem.item o r id c) o
   | reachable_right : forall o r id c, OriginReachableStep (YjsItem.item o r id c) r
 
-def OriginReachable := TransGen (r := OriginReachableStep A)
+def OriginReachable := TransGen (r := @OriginReachableStep A)
 
-inductive OriginLt : YjsPtr A -> YjsPtr A -> Prop where
-  | ltOrigin x y : OriginLtStep A x y -> OriginLt x y
+inductive OriginLt (P : @ClosedPredicate A): YjsPtr A -> YjsPtr A -> Prop where
+  | ltOrigin x y : P.val x -> P.val y -> OriginLtStep A x y -> OriginLt P x y
   /-
     if t is reachable, then t isn't between o and r
     This means that (YjsItem.item o r id c) is neightbor of l and r at least when inserted.
   -/
   | ltReachableOrigin o r id c t :
-    OriginReachable A (YjsItem.item o r id c) t ->
-    OriginLt t r ->
-    OriginLt t o
+    P.val o -> P.val r -> P.val t ->
+    @OriginReachable A (YjsItem.item o r id c) t ->
+    OriginLt P t r ->
+    OriginLt P t o
   | ltReachableRight o r id c t :
-    OriginReachable A (YjsItem.item o r id c) t ->
-    OriginLt o t ->
-    OriginLt r t
+    P.val o -> P.val r -> P.val t ->
+    @OriginReachable A (YjsItem.item o r id c) t ->
+    OriginLt P o t ->
+    OriginLt P r t
   | ltTrans : forall x y z,
-    OriginLt x y -> OriginLt y z -> OriginLt x z
+    P.val x -> P.val y -> P.val z ->
+    OriginLt P x y -> OriginLt P y z -> OriginLt P x z
 
--- Defines a subset of YjsItem which are possible DAG of a history of insertions.
+lemma origin_lt_p1 {A} {P : @ClosedPredicate A} {x y : YjsPtr A} (h : OriginLt _ P x y) : P.val x := by
+  cases h with
+  | ltOrigin x y hpx hpy hlt =>
+    assumption
+  | ltReachableOrigin o r id c t ho hr ht hreach hlt =>
+    assumption
+  | ltReachableRight o r id c t ho hr ht hreach hlt =>
+    assumption
+  | ltTrans x y z hx hy hz hlt1 hlt2 =>
+    assumption
 
-variable (P : YjsItem A -> Prop)
-
-def YjsItemSubset := { i : YjsItem A // P i }
-
-def YjsItemSubsetLt (x y : YjsItemSubset _ P) : Prop :=
-  x = y ∨ OriginLt A (↑x.1) (↑y.1)
-
-def ValidYjsSubsetPred :=
-  (∀ (o : YjsItem A) r id c, P (YjsItem.item o r id c) -> P o) ∧
-  (∀ o (r : YjsItem A) id c, P (YjsItem.item o r id c) -> P r) ∧
-  IsPartialOrder (YjsItemSubset _ P ) (YjsItemSubsetLt _ _)
+lemma origin_lt_p2 {A} {P : @ClosedPredicate A} {x y : YjsPtr A} (h : OriginLt _ P x y) : P.val y := by
+  cases h with
+  | ltOrigin  y hpx hpy hlt
+    assumption
+  | ltReachableOrigin o r id c t ho hr ht hreach hlt =>
+    assumption
+  | ltReachableRight o r id c t ho hr ht hreach hlt =>
+    assumption
+  | ltTrans x y z hx hy hz hlt1 hlt2 =>
+    assumption
