LeanYjs/YjsInvariant.lean
@@ -1,0 +1,407 @@
+import LeanYjs.Item
+import LeanYjs.ItemOriginOrder
+import LeanYjs.ActorId
+import LeanYjs.ItemOrder
+
+import Mathlib.Tactic.Set
+
+variable {A : Type} [BEq A]
+
+-- Defines a subset of YjsItem which are possible DAG of a history of insertions.
+
+variable (P : ClosedPredicate A)
+
+def ItemSet := { i : YjsItem A // P.val i }
+
+def OriginLeq' (x y : ItemSet P) : Prop :=
+  x = y ∨ OriginLt A P (↑x.1) (↑y.1)
+
+def YjsLt' (x y : ItemSet P) : Prop :=
+  ∃ h, @YjsLt A P h (↑x.1) (↑y.1)
+
+def YjsLeq' (x y : ItemSet P) : Prop :=
+  ∃ h, @YjsLeq A P h (↑x.1) (↑y.1)
+
+def YjsInvariant :=
+  forall h (x y : YjsItem A),
+    P.val x -> P.val y ->
+    @YjsLt A P h x y ->
+      (∃ h, @YjsLeq A P h x (y.origin)) ∨
+      (∃ h,  @YjsLt A P h (y.origin) (x.origin)) ∨
+      (x.origin = y.origin ∧ ((∃ h, @YjsLt A P h x.rightOrigin y) ∨ x.id < y.id))
+
+def ItemSetInvariant :=
+  P.val YjsPtr.first ∧
+  P.val YjsPtr.last ∧
+  (∀ (o : YjsPtr A) r id c, P.val (YjsItem.item o r id c) -> P.val o) ∧
+  (∀ o (r : YjsPtr A) id c, P.val (YjsItem.item o r id c) -> P.val r) ∧
+  (∀ (x y : YjsPtr A), P.val x -> P.val y -> OriginLt A P x y -> OriginLt A P y x -> False) ∧
+  YjsInvariant P
+
+lemma not_item_lt_first {A} {P : ClosedPredicate A} : ItemSetInvariant P -> ∀ h (o : YjsItem A), ¬ @YjsLt A P h o YjsPtr.first := by
+  intros hinv h o
+  apply @Nat.strongRecOn' (P := fun h => ∀ (o : YjsItem A), ¬ @YjsLt A P h o YjsPtr.first)
+  intros n ih o hlt
+  cases hlt with
+  | ltConflict h _ _ hlt =>
+    cases hlt
+  | ltOriginOrder _ _ hlt =>
+    have hlt2 : @OriginLt A P YjsPtr.first o := by
+      apply OriginLt.ltOrigin (x := YjsPtr.first) (y := YjsPtr.itemPtr o)
+      . apply hinv.1
+      . apply origin_lt_p1 at hlt; assumption
+      . apply OriginLtStep.lt_first
+    obtain ⟨ hfirst, hlast, hleft, hright, hanti, hinv ⟩ := hinv
+    apply hanti (x := YjsPtr.first) (y := o) <;> try assumption
+    apply origin_lt_p1 at hlt; assumption
+  | ltTrans h1 h2 x y z hlt1 hlt2 =>
+    have hlt_h2 : h2 < max h1 h2 + 1 := by
+      omega
+    apply ih _ hlt_h2 _ hlt2
+
+lemma not_last_lt_item {A} {P : ClosedPredicate A} : ItemSetInvariant P -> ∀ h (o : YjsItem A), ¬ @YjsLt A P h YjsPtr.last o := by
+  intros hinv h o
+  apply @Nat.strongRecOn' (P := fun h => ∀ (o : YjsItem A), ¬ @YjsLt A P h YjsPtr.last o)
+  intros n ih o hlt
+  cases hlt with
+  | ltConflict h _ _ hlt =>
+    cases hlt
+  | ltOriginOrder _ _ hlt =>
+    have hlt2 : @OriginLt A P o YjsPtr.last := by
+      apply OriginLt.ltOrigin (x := YjsPtr.itemPtr o) (y := YjsPtr.last)
+      . apply origin_lt_p2 at hlt; assumption
+      . apply hinv.2.1
+      . apply OriginLtStep.lt_last
+    obtain ⟨ hfirst, hlast, hleft, hright, hanti, hinv ⟩ := hinv
+    apply hanti (x := YjsPtr.last) (y := o) <;> try assumption
+    apply origin_lt_p2 at hlt; assumption
+  | ltTrans h1 h2 x y z hlt1 hlt2 =>
+    have hlt_h2 : h1 < max h1 h2 + 1 := by
+      omega
+    apply ih _ hlt_h2 _ hlt1
+
+lemma not_last_lt_first {A} {P : ClosedPredicate A} : ItemSetInvariant P -> ∀ h, ¬ @YjsLt A P h YjsPtr.last YjsPtr.first := by
+  intros hinv h
+  apply @Nat.strongRecOn' (P := fun h => ¬ @YjsLt A P h YjsPtr.last YjsPtr.first)
+  intros n ih hlt
+  cases hlt with
+  | ltConflict h _ _ hlt =>
+    cases hlt
+  | ltOriginOrder _ _ hlt =>
+    have hlt' : OriginLt _ P YjsPtr.first YjsPtr.last := by
+      obtain ⟨ P, ⟨ a, b, c ⟩ ⟩ := P
+      apply OriginLt.ltOrigin <;> try assumption
+      apply OriginLtStep.lt_first_last
+    obtain ⟨ hfirst, hlast, hleft, hright, hanti, hinv ⟩ := hinv
+    apply hanti (x := YjsPtr.first) (y := YjsPtr.last) <;> assumption
+  | ltTrans h1 h2 x y z hlt1 hlt2 =>
+    apply not_item_lt_first at hlt2 <;> assumption
+
+
+lemma not_first_lt_first {A} {P : ClosedPredicate A} : ItemSetInvariant P -> ∀ h, ¬ @YjsLt A P h YjsPtr.first YjsPtr.first := by
+  intros hinv h hlt
+  have h: OriginLt A P YjsPtr.first YjsPtr.first := by
+    cases hlt with
+    | ltConflict h _ _ hlt =>
+      cases hlt
+    | ltTrans h1 h2 x y z hlt1 hlt2 =>
+      apply not_item_lt_first hinv at hlt2; contradiction
+    | ltOriginOrder _ _ hlt =>
+      assumption
+  obtain ⟨ hfirst, hlast, hleft, hright, hanti, hinv ⟩ := hinv
+  apply hanti (x := YjsPtr.first) (y := YjsPtr.first) <;> try assumption
+
+lemma not_last_lt_last {A} {P : ClosedPredicate A} : ItemSetInvariant P -> ∀ h, ¬ @YjsLt A P h YjsPtr.last YjsPtr.last := by
+  intros hinv h hlt
+  have h: OriginLt A P YjsPtr.last YjsPtr.last := by
+    cases hlt with
+    | ltConflict h _ _ hlt =>
+      cases hlt
+    | ltTrans h1 h2 x y z hlt1 hlt2 =>
+      apply not_last_lt_item hinv at hlt1; contradiction
+    | ltOriginOrder _ _ hlt =>
+      assumption
+  obtain ⟨ hfirst, hlast, hleft, hright, hanti, hinv ⟩ := hinv
+  apply hanti (x := YjsPtr.last) (y := YjsPtr.last) <;> try assumption
+
+lemma not_ptr_lt_first {A} {P : ClosedPredicate A} : ItemSetInvariant P -> ∀ h (o : YjsPtr A), ¬ @YjsLt A P h o YjsPtr.first := by
+  intros hinv h o
+  cases o with
+  | itemPtr item =>
+    apply not_item_lt_first hinv
+  | first =>
+    apply not_first_lt_first hinv
+  | last =>
+    apply not_last_lt_first hinv
+
+lemma not_last_lt_ptr {A} {P : ClosedPredicate A} : ItemSetInvariant P -> ∀ h (o : YjsPtr A), ¬ @YjsLt A P h YjsPtr.last o := by
+  intros hinv h o
+  cases o with
+  | itemPtr item =>
+    apply not_last_lt_item hinv
+  | first =>
+    apply not_last_lt_first hinv
+  | last =>
+    apply not_last_lt_last hinv
+
+lemma origin_p_valid {A} {P : ClosedPredicate A} : forall (x : YjsItem A), P.val x -> P.val x.origin := by
+  intros x px
+  obtain ⟨ p, ⟨ hp, hp', hp'', hp''' ⟩ ⟩ := P
+  simp at *
+  obtain ⟨ o, r, id, c ⟩ := x
+  simp [YjsItem.origin] at *
+  tauto
+
+lemma right_origin_p_valid {A} {P : ClosedPredicate A} : forall (x : YjsItem A), P.val x -> P.val x.rightOrigin := by
+  intros x px
+  obtain ⟨ p, ⟨ hp, hp', hp'', hp''' ⟩ ⟩ := P
+  simp at *
+  obtain ⟨ o, r, id, c ⟩ := x
+  simp [YjsItem.rightOrigin] at *
+  tauto
+
+lemma yjs_item_subset_anti_symmetry_lemma1 {A} {P : ClosedPredicate A} (inv: ItemSetInvariant P) :
+  ∀ (x y : YjsItem A) (h1 h2 h3 : Nat),
+    P.val x →
+    P.val y →
+    YjsLt P h1 x y ->
+    YjsLt P h2 y x ->
+    YjsLeq P h3 (YjsPtr.itemPtr x) y.origin →
+    ∃ (x' y' : YjsItem A) (h1' h2' : Nat),
+      P.val x' ∧ P.val y' ∧
+      YjsLt P h1' x' y' ∧ YjsLt P h2' y' x' ∧ x'.size + y'.size < x.size + y.size := by
+  intro x y h1 h2 h3 hx hy hltxy hltyx hleq
+  have hpxo : P.val x.origin := by
+    apply origin_p_valid; assumption
+  have hpyo : P.val y.origin := by
+    apply origin_p_valid; assumption
+
+  have ⟨ h'', hlt' ⟩ : ∃ h'', YjsLt P h'' y.origin x := by
+    exists max 0 h2 + 1
+    apply YjsLt.ltTrans (y := y) <;> try assumption
+    apply YjsLt.ltOriginOrder
+    apply OriginLt.ltOrigin <;> try assumption
+    . obtain ⟨ o, r, id, c ⟩ := y
+      apply OriginLtStep.lt_left
+
+  have ⟨ h''', hlt'' ⟩ : ∃ h''', YjsLt P h''' x y.origin := by
+    cases hleq with
+    | inl heq =>
+      rw [<-heq]
+      rw [<-heq] at hlt'
+      exists h''
+    | inr hlt =>
+      exists h3
+
+  generalize heq : y.origin = yo at hlt' hlt'' hpxo hpyo
+  cases yo with
+  | first =>
+    apply not_item_lt_first inv at hlt''; contradiction
+  | last =>
+    apply not_last_lt_item inv at hlt'; contradiction
+  | itemPtr yo =>
+    exists x, yo, h''', h''
+    constructor; assumption
+    constructor; assumption
+    constructor; assumption
+    constructor; assumption
+    obtain ⟨ o, r, id, c ⟩ := y
+    simp [YjsItem.size, YjsItem.origin] at *
+    rw [heq] at *
+    simp [YjsPtr.size] at *
+    omega
+
+lemma yjs_item_subset_anti_symmetry_lemma2 {A} {P : ClosedPredicate A} (inv: ItemSetInvariant P) :
+  ∀ (x y : YjsItem A) (h1 h2 h3 h4 : Nat),
+    P.val x →
+    P.val y →
+    YjsLt P h1 x y ->
+    YjsLt P h2 y x ->
+    YjsLt P h3 y.origin x.origin →
+    YjsLeq P h4 x.origin y.origin →
+    ∃ (x' y' : YjsItem A) (h1' h2' : Nat),
+      P.val x' ∧ P.val y' ∧
+      YjsLt P h1' x' y' ∧ YjsLt P h2' y' x' ∧ x'.size + y'.size < x.size + y.size := by
+  intro x y h1 h2 h3 h4 hx hy hltxy hltyx hltyoxo hleqxoyo
+  have hpxo : P.val x.origin := by
+    apply origin_p_valid; assumption
+  have hpyo : P.val y.origin := by
+    apply origin_p_valid; assumption
+  have ⟨ h2', hlt2' ⟩ : ∃ h', YjsLt P h' x.origin y.origin := by
+    cases hleqxoyo with
+    | inl heq =>
+      rw [heq] at hltyoxo
+      rw [heq]
+      exists h3
+    | inr heq =>
+      exists h4
+  generalize heqxo : x.origin = xo at *
+  generalize heqyo : y.origin = yo at *
+  cases xo with
+  | first =>
+    apply not_ptr_lt_first inv at hltyoxo; contradiction
+  | last =>
+    apply not_last_lt_ptr inv at hlt2'; contradiction
+  | itemPtr xo =>
+    cases yo with
+    | first =>
+      apply not_item_lt_first inv at hlt2'; contradiction
+    | last =>
+      apply not_last_lt_item inv at hltyoxo; contradiction
+    | itemPtr yo =>
+      exists xo, yo, h2', h3
+      constructor; assumption
+      constructor; assumption
+      constructor; assumption
+      constructor; assumption
+      obtain ⟨ o, r, id, c ⟩ := x
+      obtain ⟨ yo, yr, yid, yc ⟩ := y
+
+      simp [YjsItem.size, YjsItem.origin] at *
+      rw [heqyo, heqxo] at *
+      simp [YjsPtr.size] at *
+      omega
+
+lemma yjs_item_subset_anti_symmetry_lemma3 {A} {P : ClosedPredicate A} (inv: ItemSetInvariant P) :
+  ∀ (x y : YjsItem A) (h1 h2 h3 : Nat),
+    P.val x →
+    P.val y →
+    YjsLt P h1 x y ->
+    YjsLt P h2 y x ->
+    YjsLt P h3 x.rightOrigin y ->
+    ∃ (x' y' : YjsItem A) (h1' h2' : Nat),
+      P.val x' ∧ P.val y' ∧
+      YjsLt P h1' x' y' ∧ YjsLt P h2' y' x' ∧ x'.size + y'.size < x.size + y.size := by
+  intro x y h1 h2 h3 hx hy hltxy hltyx hlt
+  have hpxro : P.val x.rightOrigin := by
+    apply right_origin_p_valid; assumption
+
+  have ⟨ h'', hlt' ⟩ : ∃ h'', YjsLt P h'' y x.rightOrigin := by
+    exists max h2 0 + 1
+    apply YjsLt.ltTrans
+    . apply hltyx
+    . apply YjsLt.ltOriginOrder
+      apply OriginLt.ltOrigin <;> try assumption
+      obtain ⟨ o, r, id, c ⟩ := x
+      apply OriginLtStep.lt_right
+
+  generalize heq : x.rightOrigin = xro at *
+  cases xro with
+  | first =>
+    apply not_item_lt_first inv at hlt'; contradiction
+  | last =>
+    apply not_last_lt_item inv at hlt; contradiction
+  | itemPtr xro =>
+    exists xro, y, h3, h''
+    constructor; assumption
+    constructor; assumption
+    constructor; assumption
+    constructor; assumption
+    obtain ⟨ o, r, id, c ⟩ := x
+    simp [YjsItem.size, YjsItem.rightOrigin] at *
+    rw [heq] at *
+    simp [YjsPtr.size] at *
+    omega
+
+lemma YjsItemSubsetAntiSymmetry' {A} {P : ClosedPredicate A} :
+  ItemSetInvariant P ->
+  ∀ (x y : ItemSet P), YjsLt' _ x y -> YjsLt' _ y x -> False := by
+  intro inv x y lt1 lt2
+  obtain ⟨ x, hx ⟩ := x
+  obtain ⟨ y, hy ⟩ := y
+  generalize hsize : x.size + y.size = size
+  revert x y
+  unfold YjsLt'; simp
+  apply Nat.strongRecOn' (P := fun size => ∀ (x : YjsItem A), P.val x -> ∀ (y : YjsItem A), P.val y -> ∀ h, @YjsLt A P h x y -> ∀ h', @YjsLt A P h' y x ->
+    x.size + y.size = size -> False) (n := size)
+  intros size ih x hx y hy h1 hltxy h2 hltyx hsize
+  cases size with
+  | zero =>
+    have hx : x.size = 0 := by omega
+    cases x with
+    | item o r id c =>
+      unfold YjsItem.size at hx
+      omega
+  | succ size =>
+    have hpx : P.val x := by
+      apply yjs_lt_p1 at hltyx; assumption
+    have hpy : P.val y := by
+      apply yjs_lt_p2 at hltyx; assumption
+    have hlt :
+      (∃ h, YjsLeq P h (YjsPtr.itemPtr x) y.origin) ∨
+      (∃ h, YjsLt P h y.origin x.origin) ∨
+      x.origin = y.origin ∧ ((∃ h, YjsLt P h x.rightOrigin (YjsPtr.itemPtr y)) ∨ x.id < y.id) := by
+      exact inv.2.2.2.2.2 h1 x y hpx hpy hltxy
+
+    have hlt2 :
+      (∃ h, YjsLeq P h (YjsPtr.itemPtr y) x.origin) ∨
+      (∃ h, YjsLt P h x.origin y.origin) ∨
+      y.origin = x.origin ∧ ((∃ h, YjsLt P h y.rightOrigin (YjsPtr.itemPtr x)) ∨ y.id < x.id) := by
+      exact inv.2.2.2.2.2 h2 y x hpy hpx hltyx
+
+    cases hlt with
+    | inl hlt =>
+      obtain ⟨ h', hlt ⟩ := hlt
+      obtain ⟨ x', y', h1', h2', hpx', hpy', hltxy', hltyx', hltsize ⟩ := yjs_item_subset_anti_symmetry_lemma1 inv x y _ _ _ hpx hpy hltxy hltyx hlt
+      apply ih (x'.size + y'.size) _ x' hpx' y' hpy' h1' hltxy' h2' hltyx' <;> omega
+    | inr hlt =>
+      cases hlt2 with
+      | inl hlt2 =>
+        obtain ⟨ h', hlt2 ⟩ := hlt2
+        obtain ⟨ x', y', h1', h2', hpx', hpy', hltxy', hltyx', hltsize ⟩ := yjs_item_subset_anti_symmetry_lemma1 inv y x _ _ _ hpy hpx hltyx hltxy hlt2
+        apply ih (x'.size + y'.size) _ x' hpx' y' hpy' h1' hltxy' h2' hltyx' <;> omega
+      | inr hlt2 =>
+        have ⟨ h', hleq ⟩ : ∃ h', YjsLeq P h' y.origin x.origin := by
+          unfold YjsLeq
+          cases hlt with
+          | inl hlt =>
+            obtain ⟨ h, hp ⟩ := hlt
+            exists h
+            right
+            assumption
+          | inr hlt =>
+            obtain ⟨ heq, _ ⟩ := hlt
+            exists 0
+            left
+            simp [heq]
+        have ⟨ h'', hleq2 ⟩ : ∃ h', YjsLeq P h' x.origin y.origin := by
+          unfold YjsLeq
+          cases hlt2 with
+          | inl hlt =>
+            obtain ⟨ h, hp ⟩ := hlt
+            exists h
+            right
+            assumption
+          | inr hlt =>
+            obtain ⟨ heq, _ ⟩ := hlt
+            exists 0
+            left
+            simp [heq]
+        cases hlt with
+        | inl hlt =>
+          obtain ⟨ h', hlt ⟩ := hlt
+          obtain ⟨ x', y', h1', h2', hpx', hpy', hltxy', hltyx', hltsize ⟩ := yjs_item_subset_anti_symmetry_lemma2 inv x y _ _ _ _ hpx hpy hltxy hltyx hlt hleq2
+          apply ih (x'.size + y'.size) _ x' hpx' y' hpy' h1' hltxy' h2' hltyx' <;> omega
+        | inr hlt =>
+          cases hlt2 with
+          | inl hlt2 =>
+            obtain ⟨ h', hlt2 ⟩ := hlt2
+            obtain ⟨ x', y', h1', h2', hpx', hpy', hltxy', hltyx', hltsize ⟩ := yjs_item_subset_anti_symmetry_lemma2 inv y x _ _ _ _ hpy hpx hltyx hltxy hlt2 hleq
+            apply ih (x'.size + y'.size) _ x' hpx' y' hpy' h1' hltxy' h2' hltyx' <;> omega
+          | inr hlt2 =>
+            obtain ⟨ heq, hlt ⟩ := hlt
+            obtain ⟨ _, hlt2 ⟩ := hlt2
+            cases hlt with
+            | inl hlt =>
+              obtain ⟨ h', hlt ⟩ := hlt
+              obtain ⟨ x', y', h1', h2', hpx', hpy', hltxy', hltyx', hltsize ⟩ := yjs_item_subset_anti_symmetry_lemma3 inv x y _ _ _ hpx hpy hltxy hltyx hlt
+              apply ih (x'.size + y'.size) _ x' hpx' y' hpy' h1' hltxy' h2' hltyx' <;> omega
+            | inr hlt =>
+              cases hlt2 with
+              | inl hlt2 =>
+                obtain ⟨ h', hlt2 ⟩ := hlt2
+                obtain ⟨ x', y', h1', h2', hpx', hpy', hltxy', hltyx', hltsize ⟩ := yjs_item_subset_anti_symmetry_lemma3 inv y x _ _ _ hpy hpx hltyx hltxy hlt2
+                apply ih (x'.size + y'.size) _ x' hpx' y' hpy' h1' hltxy' h2' hltyx' <;> omega
+              | inr hlt2 =>
+                unfold ActorId at *
+                omega
